cava/Cava/Monad/SequentialV.v
@@ -1,0 +1,296 @@
+(****************************************************************************)
+(* Copyright 2020 The Project Oak Authors                                   *)
+(*                                                                          *)
+(* Licensed under the Apache License, Version 2.0 (the "License")           *)
+(* you may not use this file except in compliance with the License.         *)
+(* You may obtain a copy of the License at                                  *)
+(*                                                                          *)
+(*     http://www.apache.org/licenses/LICENSE-2.0                           *)
+(*                                                                          *)
+(* Unless required by applicable law or agreed to in writing, software      *)
+(* distributed under the License is distributed on an "AS IS" BASIS,        *)
+(* WITHOUT WARRANTIES OR CONDITIONS OF ANY KIND, either express or implied. *)
+(* See the License for the specific language governing permissions and      *)
+(* limitations under the License.                                           *)
+(****************************************************************************)
+
+From Coq Require Import Bool.Bool.
+From Coq Require Import Strings.Ascii Strings.String.
+Require Import ExtLib.Structures.Monads.
+Require Export ExtLib.Data.Monads.IdentityMonad.
+Require Import ExtLib.Structures.Traversable.
+Export MonadNotation.
+
+Require Import Coq.Vectors.Vector.
+Require Import Coq.Bool.Bvector.
+Import VectorNotations.
+
+From Coq Require Import Fin.
+From Coq Require Import NArith.Ndigits.
+From Coq Require Import ZArith.ZArith.
+
+From Coq Require Import micromega.Lia.
+
+Require Import Cava.Cava.
+From Cava Require Import Kind.
+From Cava Require Import Signal.
+Require Import Cava.Monad.CavaClass.
+Require Import Cava.Monad.CombinationalMonad.
+
+(******************************************************************************)
+(* Loop combinator for feedback with delay.                                   *)
+(******************************************************************************)
+
+(*
+loopSeq' takes a combinational circuit f which has a pair of inputs which
+represent the current input of type A and current state of type C. This circuit
+returns a pair which represents the computed output of type B and next state
+value of type C. The list of input values for each clock tick are provided
+by the a parameter and the current state value is provided by the feedback
+parameter. The result of the loopSeq' is a list in the identity monad that
+represented the list of computed values at each tick.
+*)
+
+Local Open Scope vector_scope.
+
+(* TODO: FIX *)
+Fixpoint loopSeqV' {A B C : SignalType}
+                   (ticks: nat)
+                   (f : seqVType 1 A * seqVType 1 C -> ident (seqVType 1 B * seqVType 1 C))
+                   (a : seqVType ticks A) (feedback: seqVType ticks C)
+  : ident (seqType B) :=
+  match a with
+  | [] => ret []
+  | x :: xs =>
+    '(yL, nextState) <- f ([x], feedback) ;; (* One step of f. *)
+    let y := hd defaultSignal yL in
+    ys <- loopSeqV' f xs nextState ;; (* remaining steps of f *)
+    ret (y :: ys)
+  end.
+
+(*
+The loopSeq combinator takes a combinational circuit f which maps a pair
+representing the current input and current state to another pair
+representing the computed output and next state value. This function is used
+to compute the sequential behaviour of a circuit which uses f to iterate over
+the a inputs, using a default value for the initial state.
+*)
+
+(* TODO: FIX *)
+Definition loopSeqV {A B C : SignalType}
+                    (f : seqType A * seqType C -> ident (seqType B * seqType C))
+                    (a : seqType A)
+                    : ident (seqType B) :=
+  loopSeqV' f a [defaultCombValue C].
+
+(******************************************************************************)
+(* A boolean sequential logic interpretation for the Cava class               *)
+(******************************************************************************)
+
+Definition notBoolVec {ticks: nat} (i : Vector.t bool ticks)
+                       : ident (Vector.t bool ticks) :=
+  ret (Vector.map (fun a => negb a) i).
+
+Definition binOpV {A B C : Type} (ticks: nat)
+           (f: A -> B -> C)
+           (i : Vector.t A ticks * Vector.t B ticks)
+          : ident (Vector.t C ticks) :=
+  ret (Vector.map (fun '(a, b) => f a b) (vcombine (fst i) (snd i))).
+
+Definition lut1BoolVec (ticks: nat)
+           (f: bool -> bool) (i : Vector.t bool ticks)
+           : ident (Vector.t bool ticks) :=
+  ret (Vector.map f i).
+
+Definition lut2BoolVec (ticks: nat)
+                       (f: bool -> bool -> bool)
+                       (i : Vector.t bool ticks * Vector.t bool ticks)
+                      : ident (Vector.t bool ticks) :=
+  ret (Vector.map (fun (i : bool * bool) => let (a, b) := i in f a b)
+           (vcombine (fst i) (snd i))).
+
+Definition lut3BoolVec (ticks: nat)
+                       (f: bool -> bool -> bool -> bool)
+                       (i : Vector.t bool ticks * Vector.t bool ticks * Vector.t bool ticks)
+                       : ident (Vector.t bool ticks) :=
+  let '(aL, bL, cL) := i in
+  ret (Vector.map (fun (i : bool * bool * bool) => let '(a, b, c) := i in f a b c)
+                  (vcombine (vcombine aL bL) cL)).
+
+Definition lut4BoolVec (ticks: nat)
+                        (f: bool -> bool -> bool -> bool -> bool)
+                        (i : Vector.t bool ticks  * Vector.t bool ticks * 
+                             Vector.t bool ticks * Vector.t bool ticks)
+                        : ident (Vector.t bool ticks) :=
+  let '(aL, bL, cL, dL) := i in
+  ret (Vector.map (fun (i : bool * bool * bool * bool) =>
+            let '(a, b, c, d) := i in f a b c d)
+           (vcombine (vcombine (vcombine aL bL) cL) dL)).
+
+Definition lut5BoolVec (ticks: nat)
+                       (f: bool -> bool -> bool -> bool -> bool -> bool)
+                       (i : Vector.t bool ticks * Vector.t bool ticks * Vector.t bool ticks *
+                            Vector.t bool ticks * Vector.t bool ticks)
+                       : ident (Vector.t bool ticks) :=
+  let '(aL, bL, cL, dL, eL) := i in
+  ret (Vector.map (fun (i : bool * bool * bool * bool * bool) =>
+            let '(a, b, c, d, e) := i in f a b c d e)
+           (vcombine (vcombine (vcombine (vcombine aL bL) cL) dL) eL)).
+
+Definition lut6BoolVec (ticks: nat)
+                      (fn: bool -> bool -> bool -> bool -> bool -> bool -> bool)
+                      (i : Vector.t bool ticks * Vector.t bool ticks * Vector.t bool ticks *
+                           Vector.t bool ticks * Vector.t bool ticks * Vector.t bool ticks) :
+                      ident (Vector.t bool ticks) :=
+  let '(aL, bL, cL, dL, eL, fL) := i in
+  ret (Vector.map (fun (i : bool * bool * bool * bool * bool * bool) =>
+            let '(a, b, c, d, e, f) := i in fn a b c d e f)
+           (vcombine (vcombine (vcombine (vcombine (vcombine aL bL) cL) dL) eL) fL)).
+
+Definition muxcyBoolVec (ticks: nat)
+                        (s :  Vector.t bool ticks)
+                        (ci : Vector.t bool ticks)
+                        (di : Vector.t bool ticks)
+                        : ident ( Vector.t bool ticks) :=
+  let dici := vcombine di ci in
+  let s_dici := vcombine s dici in
+  ret (Vector.map (fun (i : bool * (bool * bool)) =>
+     let '(s, (ci, di)) := i in
+     match s with
+       | false => di
+       | true => ci
+     end) s_dici).
+
+Definition indexAtBoolVec {t: SignalType}
+                          {sz isz: nat}
+                          (ticks: nat)
+                          (i : Vector.t (Vector.t (combType t) sz) ticks)
+                          (sel : Vector.t (Bvector isz) ticks)
+                          : Vector.t (combType t) ticks :=
+  Vector.map (fun '(i, sel) => indexAtBool i sel) (vcombine i sel).
+
+Definition indexConstBoolVec {t: SignalType} {sz: nat}
+                             (ticks: nat)
+                             (i : Vector.t (Vector.t (combType t) sz) ticks)
+                             (sel : nat)
+                             : Vector.t (combType t) ticks :=
+  Vector.map (fun i => indexConstBool i sel) i.
+
+Definition sliceBoolVec {t: SignalType}
+                        {sz: nat}
+                        (ticks: nat)
+                        (startAt len : nat)
+                        (v: Vector.t (Vector.t (combType t) sz) ticks)
+                        (H: startAt + len <= sz) :
+                        Vector.t (Vector.t (combType t) len) ticks :=
+  Vector.map (fun v => sliceBool startAt len v H) v.
+
+Definition peelVecVec {t: SignalType} {s: nat}
+                      (ticks: nat)
+                      (v: Vector.t (Vector.t (combType t) s) ticks)
+                      : Vector.t (Vector.t (combType t) ticks) s :=
+ Vector.map (fun i => Vector.map (fun j => indexConstBool j i) v) (vseq 0 s).
+
+Definition unpeelVecVec {t: SignalType} {s: nat}
+                        (ticks: nat)
+                        (v: Vector.t (Vector.t (combType t) ticks) s)
+                        : Vector.t (Vector.t (combType t) s) ticks :=
+  Vector.map (fun ni => Vector.map (fun vi => indexConstBool vi ni) v) (vseq 0 ticks).
+
+Local Open Scope list_scope.
+
+Definition unsignedAddComb {m n : nat}
+                           (av : Bvector m) (bv : Bvector n) :
+                           Bvector (1 + max m n) :=
+  let a := Bv2N av in
+  let b := Bv2N bv in
+  let sumSize := 1 + max m n in
+  let sum := (a + b)%N in
+  N2Bv_sized sumSize sum.
+
+Definition unsignedAddBoolVec {m n : nat}
+                              (ticks: nat)
+                              (av : Vector.t (Bvector m) ticks)
+                              (bv : Vector.t (Bvector n) ticks) :
+                              ident (Vector.t (Bvector (1 + max m n)) ticks) :=
+  binOpV ticks unsignedAddComb (av, bv).
+
+Definition unsignedMultComb {m n : nat}
+                            (av : Bvector m) (bv : Bvector n) :
+                            Bvector (m + n) :=
+  let a := Bv2N av in
+  let b := Bv2N bv in
+  let product := (a * b)%N in
+  N2Bv_sized (m + n) product.
+
+Definition unsignedMultBoolVec {m n : nat}
+                               (ticks: nat)
+                               (av : Vector.t (Bvector m) ticks)
+                               (bv : Vector.t (Bvector n) ticks) :
+                               ident (Vector.t (Bvector (m + n)) ticks) :=
+  binOpV ticks unsignedMultComb (av, bv).
+
+Definition greaterThanOrEqualComb {m n : nat}
+                                  (av : Bvector m) (bv : Bvector n) :
+                                  bool :=
+  let a := N.to_nat (Bv2N av) in
+  let b := N.to_nat (Bv2N bv) in
+  b <=? a.
+
+Definition greaterThanOrEqualBoolVec {m n : nat}
+                                     (ticks: nat)
+                                     (av : Vector.t (Bvector m) ticks)
+                                     (bv : Vector.t (Bvector n) ticks) :
+                                     ident (Bvector ticks) :=
+  binOpV ticks greaterThanOrEqualComb (av, bv).
+
+Definition bufBoolVec (ticks: nat)
+           (i : Vector.t bool ticks) : ident (Vector.t bool ticks) :=
+  ret i.
+
+(******************************************************************************)
+(* Instantiate the Cava class for a boolean sequential logic                  *)
+(* interpretation.                                                            *)
+(******************************************************************************)
+
+ Instance SequentialVectorSemantics {ticks: nat} : Cava (seqVType ticks) :=
+  { cava := ident;
+    zero := ret (Vector.const false ticks);
+    one := ret (Vector.const true ticks);
+    defaultSignal t := Vector.const (@defaultCombValue t) ticks;
+    inv := notBoolVec;
+    and2 := binOpV ticks andb;
+    nand2 := binOpV ticks (fun a b => negb (a && b));
+    or2 := binOpV ticks orb;
+    nor2 := binOpV ticks (fun a b => negb (a || b));
+    xor2 := binOpV ticks xorb;
+    xnor2 := binOpV ticks (fun a b => negb (xorb a b));
+    buf_gate := bufBoolVec ticks;
+    lut1 := lut1BoolVec ticks;
+    lut2 := lut2BoolVec ticks;
+    lut3 := lut3BoolVec ticks;
+    lut4 := lut4BoolVec ticks;
+    lut5 := lut5BoolVec ticks;
+    lut6 := lut6BoolVec ticks;
+    xorcy := binOpV ticks xorb;
+    muxcy := muxcyBoolVec ticks;
+    peel _ _ v := peelVecVec ticks v;
+    unpeel _ _ v := unpeelVecVec ticks v;
+    indexAt t sz isz := @indexAtBoolVec t sz isz ticks;
+    indexConst t sz := @indexConstBoolVec t sz ticks;
+    slice t sz := @sliceBoolVec t sz ticks;
+    unsignedAdd m n := @unsignedAddBoolVec m n ticks;
+    unsignedMult m n := @unsignedMultBoolVec m n ticks;
+    greaterThanOrEqual m n := @greaterThanOrEqualBoolVec m n ticks;
+    instantiate _ circuit := circuit;
+    blackBox intf _ := ret (tupleInterfaceDefaultS (map port_type (circuitOutputs intf)));
+    delay k i := ret (@defaultCombValue k :: Vector.shiftout i); (* TODO: FIX *)
+    loop _ _ _ := loopSeqV;
+}.
+
+(******************************************************************************)
+(* A function to run a monadic circuit description and return the boolean     *)
+(* behavioural simulation result.                                             *)
+(******************************************************************************)
+
+Definition sequentialV {a} (circuit : cava a) : a := unIdent circuit.
